consolidate array and perm

src/lowparse/LowParse.Steel.VParse.fsti
@@ -59,10 +59,36 @@ let array_t (k: parser_kind) : Tot Type =
 [@@erasable]
 noeq
 type v (k: parser_kind) (t: Type) = {
-  array : array_t k;
+  array_perm : (A.array byte & SP.perm);
   contents : t;
-  perm: SP.perm;
+  array_perm_prf: squash (array_prop k (fst array_perm));
 }
+
+let array_of (#k: parser_kind) (#t: Type) (w: v k t) : GTot (array_t k) =
+  fst w.array_perm
+
+let perm_of (#k: parser_kind) (#t: Type) (w: v k t) : Tot SP.perm =
+  snd w.array_perm
+
+let adjacent
+  (#t1 #t2: Type)
+  (#k1 #k2: parser_kind)
+  (v1: v k1 t1)
+  (v2: v k2 t2)
+: Tot prop
+= A.adjacent (array_of v1) (array_of v2) /\
+  perm_of v1 == perm_of v2
+
+let merge_into
+  (#k1 #k2 #k: parser_kind)
+  (#t1 #t2 #t: Type)
+  (v1: v k1 t1)
+  (v2: v k2 t2)
+  (v: v k t)
+: Tot prop
+= A.merge_into (array_of v1) (array_of v2) (array_of v) /\
+  perm_of v1 == perm_of v /\
+  perm_of v2 == perm_of v
 
 val vparse_slprop
   (#k: parser_kind)
@@ -113,10 +139,12 @@ val intro_vparse
       valid p (h (AP.varrayptr a)).AP.contents
     )
     (fun h _ h' ->
-      valid p (h (AP.varrayptr a)).AP.contents /\
-      (h' (vparse p a)).perm == (h (AP.varrayptr a)).AP.perm /\
-      (h' (vparse p a)).array == (h (AP.varrayptr a)).AP.array /\
-      is_byte_repr p (h' (vparse p a)).contents (h (AP.varrayptr a)).AP.contents
+      let s' = h' (vparse p a) in
+      let s = h (AP.varrayptr a) in
+      valid p s.AP.contents /\
+      array_of s' == s.AP.array /\
+      perm_of s' == s.AP.perm /\
+      is_byte_repr p s'.contents s.AP.contents
     )
 
 val elim_vparse
@@ -130,10 +158,12 @@ val elim_vparse
     (fun _ -> AP.varrayptr a)
     (fun _ -> True)
     (fun h _ h' ->
-      valid p (h' (AP.varrayptr a)).AP.contents /\
-      (h' (AP.varrayptr a)).AP.perm == (h (vparse p a)).perm /\
-      (h' (AP.varrayptr a)).AP.array == (h (vparse p a)).array /\
-      is_byte_repr p (h (vparse p a)).contents (h' (AP.varrayptr a)).AP.contents
+      let s' = h' (AP.varrayptr a) in
+      let s = h (vparse p a) in
+      valid p s'.AP.contents /\
+      s'.AP.perm == perm_of s /\
+      s'.AP.array == array_of s /\
+      is_byte_repr p s.contents s'.AP.contents
     )
 
 val share
@@ -150,11 +180,11 @@ val share
       let s = h (vparse p a) in
       let s' = h' (vparse p a) in
       let d = h' (vparse p res) in
-      s'.array == s.array /\
-      s'.perm == SP.half_perm s.perm /\
+      array_of s' == array_of s /\
+      perm_of s' == SP.half_perm (perm_of s) /\
       s'.contents == s.contents /\
-      d.array == s.array /\
-      d.perm == SP.half_perm s.perm /\
+      array_of d == array_of s /\
+      perm_of d == SP.half_perm (perm_of s) /\
       d.contents == s.contents
     )
 
@@ -168,15 +198,15 @@ val gather
     (vparse p a1 `SE.star` vparse p a2)
     (fun res -> vparse p a1)
     (fun h ->
-      (h (vparse p a1)).array == (h (vparse p a2)).array
+      (h (vparse p a1)).array_perm == (h (vparse p a2)).array_perm
     )
     (fun h res h' ->
       let s1 = h (vparse p a1) in
       let s2 = h (vparse p a2) in
       let d = h' (vparse p a1) in
-      d.array == s1.array /\
-      d.array == s2.array /\
-      d.perm == s1.perm `SP.sum_perm` s2.perm /\
+      array_of d == array_of s1 /\
+      array_of d == array_of s2 /\
+      perm_of d == perm_of s1 `SP.sum_perm` perm_of s2 /\
       d.contents == s1.contents /\
       d.contents == s2.contents
     )
